updates

high/Veritas.Verifier.Blum.fst
@@ -4,7 +4,6 @@ open Veritas.EAC
 open FStar.Classical
 
 module S = FStar.Seq
-module SA = Veritas.SeqAux
 module E = Veritas.EAC
 module VT = Veritas.Verifier.Thread
 
@@ -1147,3 +1146,41 @@ let eac_add_set_mem_atleast_evict_set_mem (itsl: TL.eac_log) (be: ms_hashfn_dom)
   )
   else ()
   
+let lemma_add_seq_empty (itsl: its_log{I.length itsl = 0}):
+  Lemma (ensures (S.length (ts_add_seq itsl) = 0)) = 
+  ()
+
+let lemma_evict_seq_empty (itsl: its_log{I.length itsl = 0}):
+  Lemma (ensures (S.length (ts_evict_seq itsl) = 0)) = 
+  ()
+ 
+let lemma_add_seq_extend (itsl: its_log{I.length itsl > 0}):
+  Lemma (requires (is_blum_add (I.telem itsl)))
+        (ensures (let i = I.length itsl - 1 in
+                  let itsl' = I.prefix itsl i in
+                  let e = I.index itsl i in
+                  ts_add_seq itsl == 
+                  SA.append1 (ts_add_seq itsl') (blum_add_elem e))) = ()
+                                       
+let lemma_add_seq_extend2 (itsl: its_log{I.length itsl > 0}):
+  Lemma (requires (not (is_blum_add (I.telem itsl))))
+        (ensures (let i = I.length itsl - 1 in
+                  let itsl' = I.prefix itsl i in
+                  let e = I.index itsl i in
+                  ts_add_seq itsl == 
+                  ts_add_seq itsl')) = ()
+
+
+let lemma_evict_seq_extend (itsl: its_log{I.length itsl > 0}):
+  Lemma (requires (is_evict_to_blum (I.telem itsl)))
+        (ensures (let i = I.length itsl - 1 in
+                  let itsl' = I.prefix itsl i in
+                  ts_evict_seq itsl == 
+                  SA.append1 (ts_evict_seq itsl') (blum_evict_elem itsl i))) = ()
+                                       
+let lemma_evict_seq_extend2 (itsl: its_log{I.length itsl > 0}):
+  Lemma (requires (not (is_evict_to_blum (I.telem itsl))))
+        (ensures (let i = I.length itsl - 1 in
+                  let itsl' = I.prefix itsl i in
+                  ts_evict_seq itsl == 
+                  ts_evict_seq itsl')) = ()
