intermediate/Veritas.Intermediate.TSLog.fst
@@ -1,0 +1,90 @@
+module Veritas.Intermediate.TSLog
+
+let clock_sorted (#vcfg:_) (il: il_logS vcfg {verifiable il}): prop = admit()
+
+let create (#vcfg:_) (gl: verifiable_log vcfg): (itsl:its_log vcfg{g_logS_of itsl == gl}) = admit()
+
+let lemma_prefix_verifiable (#vcfg:_) (itsl: its_log vcfg) (i:nat{i <= I.length itsl}):
+  Lemma (ensures (verifiable (I.prefix itsl i) /\ clock_sorted (I.prefix itsl i))) = admit()
+
+let lemma_verifier_thread_state_extend (#vcfg:_) (ils: its_log vcfg) (i: I.seq_index ils):
+  Lemma (ensures (thread_state_post ils i == IntV.verify_step (thread_state_pre ils i) (I.index ils i))) = admit()
+
+let lemma_slot_is_merkle_points_to (#vcfg:_) (ils: its_log vcfg) (i: I.seq_index ils):
+  Lemma (ensures (slot_points_to_is_merkle_points_to (IntV.thread_store (thread_state_pre ils i)))) = admit()
+
+let to_logk (#vcfg:_) (il:its_log vcfg) 
+  : Tot (sil:SpecTS.il_vlog { same_shape il sil }) = admit()
+
+let lemma_to_logk_length (#vcfg:_) (il:its_log vcfg)
+  : Lemma (ensures I.length il = I.length (to_logk il)) = admit()
+
+let lemma_to_logk_thread_count (#vcfg:_) (il:its_log vcfg)
+  : Lemma (ensures thread_count il = SpecTS.thread_count (to_logk il))
+  = admit()
+
+let lemma_to_logk_thread_id_of (#vcfg:_) (il:its_log vcfg) (i:I.seq_index il)
+  : Lemma (ensures thread_id_of il i == SpecTS.thread_id_of (to_logk il) i)
+  = admit()
+
+let lemma_to_logk_prefix_commute (#vcfg:_) (il:its_log vcfg) (i:nat{i <= I.length il})
+  : Lemma (to_logk (I.prefix il i) == I.prefix (to_logk il) i)
+  = admit()
+
+let lemma_to_logk_state_ops (#vcfg:_) (ils:its_log vcfg)
+  : Lemma (ensures (let ilk = to_logk ils in
+                    to_state_ops ils = SpecTS.state_ops ilk))
+  = admit()
+
+let lemma_its_log_valid_step (#vcfg:_) (il:its_log vcfg) (i:I.seq_index il)
+  : Lemma (ensures Valid? (IntV.verify_step (thread_state_pre il i) (I.index il i)))
+  = admit()
+
+let lemma_valid_logs_entry (#vcfg:_) (il: its_log vcfg) (i:I.seq_index il)
+  : Lemma (ensures (IntV.valid_logS_entry (thread_state_pre il i) (I.index il i)))
+  = admit()
+
+let lemma_to_logk_index (#vcfg:_) (ils:its_log vcfg) (i:I.seq_index ils)
+  : Lemma (ensures (I.index (to_logk ils) i == to_logK_entry ils i))
+  = admit()
+
+let lemma_forall_store_ismap_extend (#vcfg:_) (il:its_log vcfg) (i:I.seq_index il)
+  : Lemma (requires (forall_store_ismap (I.prefix il i) /\ 
+                     is_map (thread_store (thread_state_post il i))))
+          (ensures (forall_store_ismap (I.prefix il (i + 1)))) = admit()
+
+let lemma_forall_vtls_rel_extend (#vcfg:_) (ils:its_log vcfg) (i:I.seq_index ils)
+  : Lemma (requires (let ils_i = I.prefix ils i in
+                     let ilk = to_logk ils in
+                     let ilk_i = I.prefix ilk i in                     
+                     forall_vtls_rel ils_i /\
+                     vtls_rel (thread_state_post ils i) 
+                              (SpecTS.thread_state_post ilk i)))
+          (ensures (let ilk = to_logk ils in
+                    let ils_i1 = I.prefix ils (i + 1) in
+                    forall_vtls_rel ils_i1)) = admit()
+
+let lemma_forall_vtls_rel_implies_spec_verifiable (#vcfg:_) (ils:its_log vcfg)
+  : Lemma (requires (forall_vtls_rel ils))
+          (ensures (let ilk = to_logk ils in
+                    SpecTS.verifiable ilk))
+  = admit()
+
+let lemma_vtls_rel_implies_spec_clock_sorted (#vcfg:_) (ils:its_log vcfg)
+  : Lemma (requires (forall_vtls_rel ils))
+          (ensures (let ilk = to_logk ils  in
+                    SpecTS.clock_sorted ilk))
+  = admit()
+
+let lemma_vtls_rel_implies_hash_verifiable (#vcfg:_) (ils:hash_verifiable_log vcfg)
+  : Lemma (requires (forall_vtls_rel ils))
+          (ensures (let ilk = to_logk ils in
+                    SpecTS.hash_verifiable ilk))
+  = admit()
+
+let lemma_empty_implies_spec_rel (#vcfg:_) (ils:its_log vcfg{I.length ils = 0})
+  : Lemma (spec_rel ils) = admit()
+
+let lemma_spec_rel_implies_prefix_spec_rel (#vcfg:_) (ils:its_log vcfg) (i:nat{i <= I.length ils})
+ : Lemma (ensures (let ils' = I.prefix ils i in
+                   spec_rel ils')) = admit()
