intermediate/Veritas.Intermediate.TSLog.fsti
@@ -188,4 +188,7 @@ let spec_rel #vcfg (ils: its_log vcfg) =
 
 val lemma_empty_implies_spec_rel (#vcfg:_) (ils:its_log vcfg{I.length ils = 0})
   : Lemma (spec_rel ils)
-  
+
+val lemma_spec_rel_implies_prefix_spec_rel (#vcfg:_) (ils:its_log vcfg) (i:nat{i <= I.length ils})
+ : Lemma (ensures (let ils' = I.prefix ils i in
+                   spec_rel ils'))
